Automata/Input.lean
@@ -333,7 +333,13 @@ def reverseInput (lis : List (Fin m → Fin b)) : List ℕ :=
 theorem reverseInput_length (lis : List (Fin m → Fin b)) : (reverseInput lis).length = m := by
   simp only [reverseInput, List.length_ofFn]
 
+theorem inputToBase_of_reverseInput (lis : List (Fin m → Fin (b + 2))) :
+   ∃ (k : ℕ), lis = padZeros k (inputToBase (b + 2) (by omega) (reverseInput lis) (reverseInput_length lis)) := by
+   sorry
 
+ theorem reverseInput_of_inputToBase (b : ℕ) (hb: b > 1) (l: List ℕ) (hm : l.length = m) :
+   reverseInput (inputToBase b hb l hm) = l := by
+   sorry
 
 /- USELESS CODES
 def digits' (b: ℕ) (n: ℕ) (h: b > 1) : List (Fin b) :=
